LoadStore.v
@@ -295,8 +295,7 @@ Proof.
 Qed.
 
 
-(* Lemma: get_deref_blks_byaddrs returns at most one alive block,
-   if offsets have two disjoint numbers *)
+(* Lemma: get_deref_blks_byaddrs returns at most one alive block. *)
 Lemma get_deref_blks_phyptr_singleton:
   forall (m:Ir.Memory.t) (m_wf:Ir.Memory.wf m) o Is cid sz bos
          (HSZ: 0 < sz)
@@ -353,6 +352,271 @@ Proof.
     apply H.
     apply PeanoNat.Nat.le_add_r.
   }
+Qed.
+
+Lemma get_deref_phy_nil_same:
+  forall m1 m2 bid mb bwid o cid ofs
+         (HGET:Some mb = Ir.Memory.get m1 bid)
+         (HWF1:Ir.Memory.wf m1)
+         (HWF2:Ir.Memory.wf m2)
+         (HSAME:Ir.Memory.get m1 bid = Ir.Memory.get m2 bid)
+         (HSZ:bwid > 0)
+         (HDEREF:Ir.get_deref m1 (Ir.pphy o nil cid) bwid = (bid, mb, ofs)::nil)
+         (HCALLTIME:Ir.Memory.calltimes m1 = Ir.Memory.calltimes m2),
+    Ir.get_deref m1 (Ir.pphy o nil cid) bwid =
+    Ir.get_deref m2 (Ir.pphy o nil cid) bwid.
+Proof.
+  intros.
+  unfold Ir.get_deref.
+  unfold Ir.get_deref_blks_phyptr.
+  assert (Ir.Memory.inbounds_blocks2 m1 [o; o + bwid] =
+            Ir.Memory.inbounds_blocks2 m2 [o; o + bwid]).
+  { eapply Ir.Memory.inbounds_blocks2_same; try eassumption.
+    remember (Ir.Memory.inbounds_blocks2 m1 [o; o + bwid]) as l.
+    symmetry in Heql.
+    dup Heql.
+    apply Ir.Memory.inbounds_blocks2_singleton in Heql0.
+    unfold Ir.get_deref in HDEREF.
+    unfold Ir.get_deref_blks_phyptr in HDEREF.
+    rewrite Heql in HDEREF.
+    destruct l.
+    { inv HDEREF. }
+    { destruct l.
+      { des_ifs. simpl in HDEREF. des_ifs. simpl in HDEREF. inv HDEREF.
+        destruct p. reflexivity.
+        simpl in HDEREF. inv HDEREF. destruct p. reflexivity.
+        simpl in HDEREF. inv HDEREF. destruct p. reflexivity.
+      }
+      { simpl in Heql0. omega. }
+    }
+    assumption. omega.
+  }
+  rewrite H.
+  destruct (Ir.Memory.inbounds_blocks2 m2 [o; o + bwid]); try reflexivity.
+  destruct cid; try reflexivity.
+  unfold Ir.Memory.calltime. rewrite HCALLTIME.
+  des_ifs.
+Qed.
+
+Lemma get_deref_phy_I_cons:
+  forall m bid mb bwid o cid ofs I i
+         (HGET:Some mb = Ir.Memory.get m bid)
+         (HWF1:Ir.Memory.wf m)
+         (HSZ:bwid > 0)
+         (HDEREF:Ir.get_deref m (Ir.pphy o I cid) bwid = (bid, mb, ofs)::nil),
+    (in_range i (Ir.MemBlock.P0_range mb) = true ->
+     Ir.get_deref m (Ir.pphy o (i::I) cid) bwid = (bid, mb, ofs)::nil) /\
+    (in_range i (Ir.MemBlock.P0_range mb) = false ->
+     Ir.get_deref m (Ir.pphy o (i::I) cid) bwid = nil).
+Proof.
+  intros.
+  unfold Ir.get_deref in *.
+  unfold Ir.get_deref_blks_phyptr in *.
+  remember (Ir.Memory.inbounds_blocks2 m (o :: o + bwid :: I)) as inbs1.
+  remember (Ir.Memory.inbounds_blocks2 m (o :: o + bwid :: i :: I)) as inbs2.
+  assert (Ir.Memory.inbounds_blocks2 m (o :: o + bwid :: i :: I) =
+          Ir.Memory.inbounds_blocks2 m (i :: o :: o + bwid :: I)).
+  { eapply Ir.Memory.inbounds_blocks2_Permutation with (I := i::o::(o+bwid)::I).
+    apply perm_trans with (l' := o::i::o+bwid::I).
+    constructor. apply perm_skip. constructor.
+    reflexivity. }
+  rewrite H in *. clear H.
+  dup Heqinbs1. (* make sigleton *)
+  symmetry in Heqinbs0.
+  apply Ir.Memory.inbounds_blocks2_singleton2 in Heqinbs0.
+  destruct inbs1. inv HDEREF.
+  destruct inbs1; try (simpl in Heqinbs0; omega).
+  (* okay, it is singleton. *)
+  dup Heqinbs1.
+  symmetry in Heqinbs1.
+  destruct p.
+  apply Ir.Memory.inbounds_blocks2_cons with (i := i) in Heqinbs1.
+  destruct Heqinbs1.
+  (* okay, let's destruct cid now. *)
+  destruct cid.
+  { destruct (Ir.Memory.calltime m c) eqn:HCT.
+    { simpl in HDEREF.
+      destruct (Ir.MemBlock.alive_before t0 t) eqn:HALIVE.
+      { (* okay, ready. *)
+        simpl in HDEREF. inv HDEREF.
+        split.
+        { (* inbounds *)
+          intros HINB. apply H in HINB. rewrite HINB.
+          simpl. rewrite HALIVE. simpl. reflexivity. }
+        { (* ot inbounds *)
+          intros HNOTINB. apply H0 in HNOTINB. rewrite HNOTINB.
+          reflexivity. }
+      }
+      { (* okay, ready. *)
+        simpl in HDEREF. inv HDEREF. }
+    }
+    {
+      simpl in HDEREF. inv HDEREF.
+      split.
+      { (* inbounds *)
+        intros HINB. apply H in HINB. rewrite HINB.
+        simpl. reflexivity. }
+      { (* ot inbounds *)
+        intros HNOTINB. apply H0 in HNOTINB. rewrite HNOTINB.
+        reflexivity. }
+    }
+  }
+  {
+    simpl in HDEREF. inv HDEREF.
+    split.
+    { (* inbounds *)
+      intros HINB. apply H in HINB. rewrite HINB.
+      simpl. reflexivity. }
+    { (* ot inbounds *)
+      intros HNOTINB. apply H0 in HNOTINB. rewrite HNOTINB.
+      reflexivity. }
+  }
+  assumption.
+  omega.
+Qed.
+
+Lemma get_deref_phy_I_cons2:
+  forall m bid mb bwid o cid I i
+         (HGET:Some mb = Ir.Memory.get m bid)
+         (HWF1:Ir.Memory.wf m)
+         (HSZ:bwid > 0)
+         (HDEREF:Ir.get_deref m (Ir.pphy o I cid) bwid = nil),
+     Ir.get_deref m (Ir.pphy o (i::I) cid) bwid = nil.
+Proof.
+  intros.
+  unfold Ir.get_deref in *.
+  unfold Ir.get_deref_blks_phyptr in *.
+  assert ( Ir.Memory.inbounds_blocks2 m (o :: o + bwid :: i :: I) =
+           Ir.Memory.inbounds_blocks2 m (i :: o :: o + bwid :: I)).
+  { apply Ir.Memory.inbounds_blocks2_Permutation with (I := i::o::o+bwid::I).
+    eapply perm_trans. eapply perm_swap. eapply perm_skip.
+    eapply perm_swap. reflexivity. }
+  rewrite H in *. clear H.
+
+  destruct (Ir.Memory.inbounds_blocks2 m (o::o+bwid::I)) eqn:Hib2.
+  { apply Ir.Memory.inbounds_blocks2_cons2 with (i := i) in Hib2. rewrite Hib2.
+    reflexivity.
+  }
+  { dup Hib2.
+    apply Ir.Memory.inbounds_blocks2_singleton2 in Hib0; try congruence; try omega.
+    destruct l; try (simpl in Hib0; omega).
+    destruct p.
+    apply Ir.Memory.inbounds_blocks2_cons with (i := i) in Hib2.
+    destruct Hib2.
+    destruct (in_range i (Ir.MemBlock.P0_range t)).
+    { exploit H. reflexivity. intros HH. rewrite HH.
+      rewrite HDEREF. reflexivity. }
+    { exploit H0. reflexivity. intros HH. rewrite HH.
+      reflexivity. }
+  }
+Qed.
+  
+Lemma get_deref_phy_same:
+  forall m1 m2 bid mb bwid o cid ofs I
+         (HGET:Some mb = Ir.Memory.get m1 bid)
+         (HWF1:Ir.Memory.wf m1)
+         (HWF2:Ir.Memory.wf m2)
+         (HSAME:Ir.Memory.get m1 bid = Ir.Memory.get m2 bid)
+         (HSZ:bwid > 0)
+         (HDEREF:Ir.get_deref m1 (Ir.pphy o I cid) bwid = (bid, mb, ofs)::nil)
+         (HCALLTIME:Ir.Memory.calltimes m1 = Ir.Memory.calltimes m2),
+    Ir.get_deref m1 (Ir.pphy o I cid) bwid =
+    Ir.get_deref m2 (Ir.pphy o I cid) bwid.
+Proof.
+  intros.
+  induction I.
+  { eapply get_deref_phy_nil_same; try eassumption. }
+  { remember (Ir.get_deref m1 (Ir.pphy o I cid) bwid) as bb.
+    symmetry in Heqbb.
+    dup Heqbb.
+    apply Ir.get_deref_singleton in Heqbb.
+    destruct Heqbb.
+    { (* get m1 (fst (fst bo)) is [x]. *)
+      destruct H. destruct H.
+      destruct bb. inv H.
+      destruct bb.
+      { inv H.
+        destruct x. destruct p. simpl in H0.
+        apply get_deref_phy_I_cons with (i := a) in Heqbb0; try congruence.
+        destruct Heqbb0.
+        destruct (in_range a (Ir.MemBlock.P0_range t)) eqn:HINR.
+        { exploit H. reflexivity. intros HH.
+          dup HDEREF. rewrite HH in HDEREF0. inv HDEREF0.
+          rewrite HDEREF.
+          exploit IHI. reflexivity. intros HH'. symmetry in HH'.
+          apply get_deref_phy_I_cons with (i := a) in HH'; try congruence.
+          destruct HH'. rewrite H2. reflexivity. congruence.
+        }
+        { exploit H1. reflexivity. intros HH.
+          dup HDEREF. rewrite HH in HDEREF0. inv HDEREF0. }
+      }
+      { inv H. }
+    }
+    { rewrite H in Heqbb0.
+      eapply get_deref_phy_I_cons2 with (i := a) in Heqbb0; try eassumption.
+      congruence.
+    }
+    { eassumption. }
+    { omega. }
+  }
+Qed.
+
+Lemma get_deref_blks_phyptr_inbounds_blocks2:
+  forall b t m o Is cid sz
+         (HIN:List.In (b, t) (Ir.get_deref_blks_phyptr m o Is cid sz)),
+    List.In (b, t) (Ir.Memory.inbounds_blocks2 m (o::o+sz::Is)).
+Proof.
+  intros.
+  unfold Ir.get_deref_blks_phyptr in HIN.
+  des_ifs.
+  { eapply List.filter_In. eassumption. }
+Qed.
+
+Theorem get_deref_phy_singleton:
+  forall (m:Ir.Memory.t) (m_wf:Ir.Memory.wf m) o Is cid (sz:nat) bos
+         (HSZ: 0 < sz)
+         (HDEREF: Ir.get_deref m (Ir.pphy o Is cid) sz = bos),
+  (exists bo, bos = bo::nil /\
+              Ir.Memory.get m bo.(fst).(fst) = Some bo.(fst).(snd) /\
+              o = Ir.MemBlock.addr (bo.(fst).(snd)) + (bo.(snd)))
+  \/ (bos = nil).
+Proof.
+  intros.
+  unfold Ir.get_deref in HDEREF.
+  remember (Ir.get_deref_blks_phyptr m o Is cid sz) as blks.
+  assert ((exists bo0, blks = bo0::nil /\
+                       Ir.Memory.get m bo0.(fst) = Some bo0.(snd))
+          \/ (blks = nil)).
+  { eapply Ir.get_deref_blks_phyptr_singleton.
+    eassumption.
+    eassumption.
+    rewrite <- Heqblks. reflexivity. }
+  destruct H.
+  { destruct H.
+    destruct H.
+    rewrite H in HDEREF.
+    simpl in HDEREF.
+    left. eexists. split. rewrite <- HDEREF.
+    reflexivity. simpl.
+    split. assumption.
+    destruct x. simpl in *.
+    assert (Ir.MemBlock.addr t <= o).
+    { assert (List.In (b, t) blks).
+      { rewrite H. simpl. left. reflexivity. }
+      rewrite Heqblks in H1.
+      apply get_deref_blks_phyptr_inbounds_blocks2 in H1.
+      remember (Ir.Memory.inbounds_blocks2 m (o :: o + sz :: Is)) as lt.
+      symmetry in Heqlt.
+      dup Heqlt.
+      apply In_pair_split_snd in H1.
+      apply Ir.Memory.inbounds_blocks2_forallb in Heqlt.
+      eapply forallb_In in Heqlt; try eassumption.
+      SearchAbout Ir.MemBlock.addr.
+      eapply Ir.MemBlock.inbounds_abs_addr in Heqlt. omega. reflexivity.
+    }
+    omega.
+  }
+  { right. rewrite H in HDEREF. simpl in HDEREF. congruence. }
 Qed.
 
 (* Theorem: get_deref always returns at most one block. *)
